compiler/src/examples/Fibonacci.v
@@ -75,16 +75,11 @@ Definition do_regalloc: bool := false.
 
 Definition compileFunc: cmd -> list Instruction :=
   if do_regalloc then
-    (fun s => snd (exprImp2Riscv_with_regalloc Lw Sw Demos.Fibonacci.b s))
+    (fun s => exprImp2Riscv_with_regalloc Lw Sw Demos.Fibonacci.b s)
   else
     (exprImp2Riscv Lw Sw).
 
-(* register, actually *)
-Definition resVar :=
-  if do_regalloc then
-    fst (exprImp2Riscv_with_regalloc Lw Sw Demos.Fibonacci.b (fib_ExprImp 6))
-  else
-    Demos.Fibonacci.b.
+Definition resVar := Demos.Fibonacci.b.
 
 Definition fib_riscv0(n: Z): list Instruction :=
   compileFunc (fib_ExprImp n).
@@ -122,7 +117,8 @@ Module PrintRegAllocAnnotatedFlatImp.
              riscvRegisters
              empty_map
              flat
-             (@singleton_set var _ resVar).
+             empty_set
+             (interesting_alloc resVar).
 
   Definition regAllocWithCheck flat resVar :=
     checker var var func empty_map (regAlloc flat resVar).
@@ -146,6 +142,7 @@ let r := eval cbv in (regAllocWithCheck (flatten (fib_ExprImp 6)) Demos.Fibonacc
     end.
     let b := eval unfold checker in checker in change checker with b.
     cbv beta iota.
+    (*
     match goal with
     | |- context [ loop_inv var var func ?ma ?m ?s1 ?s2 ] =>
       let i := constr:(loop_inv var var func ma m s1 s2) in
@@ -173,38 +170,7 @@ let r := eval cbv in (regAllocWithCheck (flatten (fib_ExprImp 6)) Demos.Fibonacc
                  (ASSeq Z Z Z (ASLit Z Z Z 9 5 6) (ASOp Z Z Z 10 6 ltu 8 9))))).
       Open Scope regalloc_scope.
       simpl (mappings var var func _ _).
-      (*
-        case SLoop of regalloc is wrong, it should not only pass (union l (live s))
-        to the recursive call, but also mandate that they will be stored in the same
-        registers as before!
-
-              let s2' := regalloc (mappings m s1') s2 (union l (live s)) in
-
-(($x5($r1) = 0;
-  $x1($r2) = $x5);
- ($x6($r1) = 1;
-  $x2($r3) = $x6);
- ($x7($r1) = 0;
-  $x4($r4) = $x7);
- loop
-      ($x8($r1) = $x4;
-       $x9($r5) = 6;
-       $x10($r6) = ltu $x8 $x9)
-      breakUnless $x10
-      ((($x11($r1) = $x1;
-         $x12($r2) = $x2;
-         $x13($r5) = add $x11 $x12);
-        $x3($r1) = $x13);
-       ($x14($r2) = $x2;
-        $x1($r3) = $x14);
-       ($x15($r2) = $x3;
-        $x2($r1) = $x15);
-       ($x16($r2) = $x4;
-        $x17($r4) = 1;
-        $x18($r5) = add $x16 $x17);
-       $x4($r2) = $x18))
-
-checker seems correct, regalloc is wrong *)
+      *)
   Abort.
 End PrintRegAllocAnnotatedFlatImp.
 
